Complete Milestone 4 receipt semantics

Oracle/contracts/async.wat
@@ -1,0 +1,88 @@
+(module
+  (import "env" "input" (func $input (param i64)))
+  (import "env" "current_account_id" (func $current_account_id (param i64)))
+  (import "env" "register_len" (func $register_len (param i64) (result i64)))
+  (import "env" "read_register" (func $read_register (param i64 i64)))
+  (import "env" "value_return" (func $value_return (param i64 i64)))
+  (import "env" "promise_create"
+    (func $promise_create
+      (param i64 i64 i64 i64 i64 i64 i64 i64)
+      (result i64)))
+  (import "env" "promise_then"
+    (func $promise_then
+      (param i64 i64 i64 i64 i64 i64 i64 i64 i64)
+      (result i64)))
+  (import "env" "promise_return" (func $promise_return (param i64)))
+  (import "env" "promise_result" (func $promise_result (param i64 i64) (result i64)))
+
+  (memory (export "memory") 1)
+  (data (i32.const 0) "echo")
+  (data (i32.const 8) "callback")
+  (data (i32.const 24) "\07")
+
+  (func (export "call_then") (local $target_len i64) (local $self_len i64)
+    (local $promise i64) (local $callback i64)
+    i64.const 0
+    call $input
+    i64.const 0
+    call $register_len
+    local.set $target_len
+    i64.const 0
+    i64.const 64
+    call $read_register
+    local.get $target_len
+    i64.const 64
+    i64.const 4
+    i64.const 0
+    i64.const 0
+    i64.const 0
+    i64.const 32
+    i64.const 30000000000000
+    call $promise_create
+    local.set $promise
+    i64.const 1
+    call $current_account_id
+    i64.const 1
+    call $register_len
+    local.set $self_len
+    i64.const 1
+    i64.const 128
+    call $read_register
+    local.get $promise
+    local.get $self_len
+    i64.const 128
+    i64.const 8
+    i64.const 8
+    i64.const 0
+    i64.const 0
+    i64.const 32
+    i64.const 30000000000000
+    call $promise_then
+    local.set $callback
+    local.get $callback
+    call $promise_return)
+
+  (func (export "echo")
+    i64.const 1
+    i64.const 24
+    call $value_return)
+
+  (func (export "callback") (local $status i64) (local $length i64)
+    i64.const 0
+    i64.const 0
+    call $promise_result
+    local.set $status
+    local.get $status
+    i64.const 1
+    i64.eq
+    if
+      i64.const 0
+      call $register_len
+      local.set $length
+      i64.const 0
+      i64.const 256
+      call $read_register
+      local.get $length
+      i64.const 256
+      call $value_return
+    end))
